wip

src/drf/DRF_PF.v
@@ -1441,278 +1441,1466 @@ Qed.
 
 Section MAPPED.
 
-  Inductive map_preserving (P: Loc.t -> Time.t -> Prop) (f: Loc.t -> Time.t -> Time.t) :=
-  | map_preserving_intro
-      (PRSVLT: forall loc t0 t1 (SAT0: P loc t0) (SAT1: P loc t1) (LT: Time.le t0 t1),
-          Time.le (f loc t0) (f loc t1))
-      (PRSVBOT: forall loc, f loc Time.bot = Time.bot)
-  .
+  Variable f: Loc.t -> Time.t -> Time.t -> Prop.
+  Hypothesis map_le:
+    forall loc t0 t1 ft0 ft1
+           (MAP0: f loc t0 ft0)
+           (MAP1: f loc t1 ft1),
+      Time.le t0 t1 -> Time.le ft0 ft1.
+  Hypothesis map_bot:
+    forall loc,
+      f loc Time.bot Time.bot.
+  Hypothesis map_eq:
+    forall loc to ft0 ft1
+           (MAP0: f loc to ft0)
+           (MAP1: f loc to ft1),
+      ft0 = ft1.
 
-  Notation collapsed f := (fun loc t0 t1 => f loc t0 = f loc t1).
-  (* Definition collapsed (f: Loc.t -> Time.t -> Time.t) (loc: Loc.t) (t0 t1: Time.t): Prop := *)
+  Definition dom loc to: Prop :=
+    exists fto, f loc to fto.
+
+  Definition collapsed (loc: Loc.t) (t0 t1: Time.t): Prop :=
+    exists ft,
+      (<<MAP0: f loc t0 ft>>) /\ (<<MAP1: f loc t1 ft>>).
+
+  (* Definition collapsed (loc: Loc.t) (t0 t1: Time.t): Prop := *)
   (*   f loc t0 = f loc t1. *)
 
-  Global Program Instance collapsed_Equivalence (f: Loc.t -> Time.t -> Time.t) loc:
-    Equivalence (collapsed f loc).
-  Next Obligation.
-  Proof.
-    ii. etrans; eauto.
-  Qed.
+  (* Global Program Instance collapsed_Equivalence loc: *)
+  (*   Equivalence (collapsed loc). *)
+  (* Next Obligation. *)
+  (* Proof. *)
+  (*   unfold collapsed. ii. ss. *)
+  (* Qed. *)
+  (* Next Obligation. *)
+  (* Proof. *)
+  (*   unfold collapsed. ii. ss. *)
+  (* Qed. *)
+  (* Next Obligation. *)
+  (* Proof. *)
+  (*   unfold collapsed. ii. etrans; eauto. *)
+  (* Qed. *)
 
-  Definition map_preserving_le_if P f
-             (PRSV: map_preserving P f)
-             loc t0 t1
-             (SAT0: P loc t0) (SAT1: P loc t1)
-    :
-      Time.le t0 t1 -> Time.le (f loc t0) (f loc t1).
-  Proof.
-    inv PRSV. eauto.
-  Qed.
-  Hint Resolve map_preserving_le_if.
-
-  Definition map_preserving_bot P f
-             (PRSV: map_preserving P f)
-             loc
-    :
-      f loc Time.bot = Time.bot.
-  Proof.
-    inv PRSV. eauto.
-  Qed.
-  Hint Resolve map_preserving_bot.
-
-  Lemma collapsed_inside P f
-        (PRSV: map_preserving P f)
-        loc t0 t3
-        (SAT0: P loc t0) (SAT3: P loc t3)
-        (CLPS: collapsed f loc t0 t3)
-        t1 t2
-        (SAT1: P loc t1)
-        (SAT2: P loc t2)
+  Lemma collapsed_inside
+        loc
+        t0 t1 t2 t3
+        ft0 ft1 ft2 ft3
+        (MAP0: f loc t0 ft0)
+        (MAP1: f loc t1 ft1)
+        (MAP2: f loc t2 ft2)
+        (MAP3: f loc t3 ft3)
+        (CLPS: collapsed loc t0 t3)
         (TLE0: Time.le t0 t1)
         (TLE1: Time.le t1 t2)
         (TLE2: Time.le t2 t3)
     :
-      collapsed f loc t1 t2.
+      collapsed loc t1 t2.
   Proof.
-    eapply map_preserving_le_if in TLE0; eauto.
-    eapply map_preserving_le_if in TLE1; eauto.
-    eapply map_preserving_le_if in TLE2; eauto.
-    ss. eapply TimeFacts.antisym; eauto.
-    etrans; eauto. rewrite <- CLPS. eauto.
+    eapply map_le in TLE0; eauto.
+    eapply map_le in TLE1; eauto.
+    eapply map_le in TLE2; eauto.
+    unfold collapsed in *. des.
+    hexploit (map_eq MAP0 MAP4). i. subst.
+    hexploit (map_eq MAP3 MAP5). i. subst.
+    exploit TimeFacts.antisym; eauto. i. subst.
+    exploit TimeFacts.antisym; eauto. i. subst.
+    esplits; eauto.
   Qed.
 
-  Lemma not_collapsed_outside P f
-        (PRSV: map_preserving P f)
-        loc t1 t2
-        (SAT1: P loc t1) (SAT2: P loc t2)
-        (TLE1: Time.le t1 t2)
-        (NCLPS: ~ collapsed f loc t1 t2)
-        t0 t3
-        (SAT0: P loc t0)
-        (SAT3: P loc t3)
+  Lemma not_collapsed_outside
+        loc
+        t0 t1 t2 t3
+        ft0 ft1 ft2 ft3
+        (MAP0: f loc t0 ft0)
+        (MAP1: f loc t1 ft1)
+        (MAP2: f loc t2 ft2)
+        (MAP3: f loc t3 ft3)
+        (NCLPS: ~ collapsed loc t1 t2)
         (TLE0: Time.le t0 t1)
+        (TLE1: Time.le t1 t2)
         (TLE2: Time.le t2 t3)
     :
-      ~ collapsed f loc t0 t3.
+      ~ collapsed loc t0 t3.
   Proof.
     ii. apply NCLPS. eapply collapsed_inside.
-    - apply PRSV.
-    - apply SAT0.
-    - apply SAT3.
-    - apply H.
-    - apply SAT1.
-    - apply SAT2.
-    - apply TLE0.
-    - apply TLE1.
-    - apply TLE2.
+    - apply MAP0.
+    - apply MAP1.
+    - apply MAP2.
+    - apply MAP3.
+    - auto.
+    - auto.
+    - auto.
+    - auto.
   Qed.
 
-  Lemma map_preserving_lt_only_if P f
-             (PRSV: map_preserving P f)
-             loc t0 t1
-             (SAT0: P loc t0) (SAT1: P loc t1)
+  Lemma map_lt_only_if
+        loc t0 t1 ft0 ft1
+        (MAP0: f loc t0 ft0)
+        (MAP1: f loc t1 ft1)
     :
-      Time.lt (f loc t0) (f loc t1) -> Time.lt t0 t1.
+      Time.lt ft0 ft1 -> Time.lt t0 t1.
   Proof.
-    inv PRSV.
     set (DenseOrder.DenseOrderFacts.OrderTac.TO.lt_total t0 t1). des; eauto.
-    - clarify. i. timetac.
-    - exploit PRSVLT.
-      + eapply SAT1.
-      + eapply SAT0.
+    - clarify. i.
+      hexploit (map_eq MAP0 MAP1). i. subst.
+      timetac.
+    - exploit map_le.
+      + eapply MAP1.
+      + eapply MAP0.
       + left. eauto.
       + i. timetac.
   Qed.
-  Hint Resolve map_preserving_lt_only_if.
+  Hint Resolve map_lt_only_if.
 
-  Definition map_preserving_lt_iff P f
-             (PRSV: map_preserving P f)
-             loc t0 t1
-             (SAT0: P loc t0) (SAT1: P loc t1)
-             (CLPS: ~ collapsed f loc t0 t1)
+  Definition map_eq_iff
+             loc t0 t1 ft0 ft1
+             (MAP0: f loc t0 ft0)
+             (MAP1: f loc t1 ft1)
+             (CLPS: ~ collapsed loc t0 t1)
     :
-      Time.lt t0 t1 <-> Time.lt (f loc t0) (f loc t1).
-  Proof.
-    split; i; cycle 1.
-    { eapply map_preserving_lt_only_if; eauto. }
-    inv PRSV. exploit PRSVLT.
-    - eapply SAT0.
-    - eapply SAT1.
-    - left. eauto.
-    - i. destruct x; auto.
-      apply CLPS in H0. des; timetac.
-  Qed.
-  Hint Resolve map_preserving_lt_iff.
-
-  Definition map_preserving_eq_iff P f
-             (PRSV: map_preserving P f)
-             loc t0 t1
-             (SAT0: P loc t0) (SAT1: P loc t1)
-             (CLPS: ~ collapsed f loc t0 t1)
-    :
-      t0 = t1 <-> (f loc t0) = (f loc t1).
+      t0 = t1 <-> ft0 = ft1.
   Proof.
     split; i; clarify; eauto.
+    exfalso. apply CLPS. eexists. eauto.
   Qed.
-  Hint Resolve map_preserving_eq_iff.
+  Hint Resolve map_eq_iff.
 
-  Definition map_preserving_le_iff P f
-             (PRSV: map_preserving P f)
-             loc t0 t1
-             (SAT0: P loc t0) (SAT1: P loc t1)
-             (CLPS: ~ collapsed f loc t0 t1)
+  Definition map_lt_iff
+             loc t0 t1 ft0 ft1
+             (MAP0: f loc t0 ft0)
+             (MAP1: f loc t1 ft1)
+             (CLPS: ~ collapsed loc t0 t1)
     :
-      Time.le t0 t1 <-> Time.le (f loc t0) (f loc t1).
+      Time.lt t0 t1 <-> Time.lt ft0 ft1.
+  Proof.
+    split; i; cycle 1.
+    { eapply map_lt_only_if; eauto. }
+    exploit map_le.
+    - eapply MAP0.
+    - eapply MAP1.
+    - left. eauto.
+    - i. destruct x; auto. exfalso. apply CLPS.
+      destruct H0. eexists. eauto.
+  Qed.
+  Hint Resolve map_lt_iff.
+
+  Definition map_le_iff
+             loc t0 t1 ft0 ft1
+             (MAP0: f loc t0 ft0)
+             (MAP1: f loc t1 ft1)
+             (CLPS: ~ collapsed loc t0 t1)
+    :
+      Time.le t0 t1 <-> Time.le ft0 ft1.
   Proof.
     repeat rewrite DenseOrder.DenseOrder.le_lteq.
     split; i; des; clarify; eauto.
-    left. erewrite <- map_preserving_lt_iff; eauto.
+    - left. erewrite <- map_lt_iff; eauto.
+    - right. eapply map_eq_iff; eauto.
   Qed.
-  Hint Resolve map_preserving_le_iff.
+  Hint Resolve map_le_iff.
 
-  Definition timemap_map (f: Loc.t -> Time.t -> Time.t) (tm: TimeMap.t): TimeMap.t :=
-    fun l => f l (tm l).
+  Definition timemap_map (tm ftm: TimeMap.t): Prop :=
+    forall loc, f loc (tm loc) (ftm loc).
 
-  Definition view_map (f: Loc.t -> Time.t -> Time.t) (v: View.t): View.t :=
-    View.mk (timemap_map f v.(View.pln)) (timemap_map f v.(View.rlx)).
 
-  Definition tview_map (f: Loc.t -> Time.t -> Time.t) (v: TView.t): TView.t :=
-    TView.mk
-      (fun loc => view_map f (v.(TView.rel) loc))
-      (view_map f v.(TView.cur))
-      (view_map f v.(TView.acq)).
+  Record view_map (vw fvw: View.t): Prop :=
+    view_map_intro
+      { map_pln: timemap_map vw.(View.pln) fvw.(View.pln);
+        map_rlx: timemap_map vw.(View.rlx) fvw.(View.rlx);
+      }.
 
-  Definition msg_map (f: Loc.t -> Time.t -> Time.t) (msg: Message.t): Message.t :=
-    match msg with
-    | Message.reserve => Message.reserve
-    | Message.full val released =>
-      Message.full val (option_map (view_map f) released)
-    end.
+  (* Inductive view_map (vw fvw: View.t): Prop := *)
+  (* | view_map_intro *)
+  (*     (PLN: timemap_map vw.(View.pln) fvw.(View.pln)) *)
+  (*     (RLX: timemap_map vw.(View.rlx) fvw.(View.rlx)) *)
+  (* . *)
 
-  Definition tevent_map (f: Loc.t -> Time.t -> Time.t) (te: ThreadEvent.t): ThreadEvent.t :=
-    match te with
-    | ThreadEvent.promise loc from to msg kind =>
-      ThreadEvent.promise loc (f loc from) (f loc to) (msg_map f msg) kind
-    | ThreadEvent.read loc to val v o =>
-      ThreadEvent.read loc (f loc to) val (option_map (view_map f) v) o
-    | ThreadEvent.write loc to from val v o =>
-      ThreadEvent.write loc (f loc to) (f loc from) val (option_map (view_map f) v) o
-    | ThreadEvent.update loc to from valr valw vr vw or ow =>
-      ThreadEvent.update loc (f loc to) (f loc from) valr valw (option_map (view_map f) vr) (option_map (view_map f) vw) or ow
-    | ThreadEvent.fence or ow => ThreadEvent.fence or ow
-    | ThreadEvent.syscall e => ThreadEvent.syscall e
-    | _ => te
-    end.
-
-  Inductive memory_map f m_src m_tgt: Prop :=
-  | memory_map_intro
-      (MAPPED: forall loc to from msg (GET: Memory.get loc to m_tgt = Some (from, msg)),
-          Memory.get loc (f loc to) m_src = Some (f loc from, msg_map f msg))
-      (ONLY: forall loc to_src msg_src (GET: Memory.get loc to_src m_src = Some msg_src),
-          exists to msg,
-            (<<FROM: f loc to = to_src>>) /\
-            (<<GET: Memory.get loc to m_tgt = Some msg>>))
+  Inductive opt_view_map: option View.t -> option View.t -> Prop :=
+  | opt_view_map_some
+      vw fvw
+      (MAP: view_map vw fvw)
+    :
+      opt_view_map (Some vw) (Some fvw)
+  | opt_view_map_none
+    :
+      opt_view_map None None
   .
 
-  Lemma map_time_join P f loc t0 t1
-        (PRSV: map_preserving P f)
-        (SAT0: P loc t0) (SAT1: P loc t1)
+  Record tview_map (vw fvw: TView.t): Prop :=
+    tview_map_intro
+      { map_rel: forall loc, view_map (vw.(TView.rel) loc) (fvw.(TView.rel) loc);
+        map_cur: view_map vw.(TView.cur) fvw.(TView.cur);
+        map_acq: view_map vw.(TView.acq) fvw.(TView.acq);
+      }.
+
+  (* Inductive tview_map (vw fvw: TView.t): Prop := *)
+  (* | tview_map_intro *)
+  (*     (REL: forall loc, view_map (vw.(TView.rel) loc) (fvw.(TView.rel) loc)) *)
+  (*     (CUR: view_map vw.(TView.cur) fvw.(TView.cur)) *)
+  (*     (ACQ: view_map vw.(TView.acq) fvw.(TView.acq)) *)
+  (* . *)
+
+  Inductive msg_map: Message.t -> Message.t -> Prop :=
+  | msg_map_reserve
     :
-      f loc (Time.join t0 t1) = Time.join (f loc t0) (f loc t1).
+      msg_map Message.reserve Message.reserve
+  | msg_map_full
+      val released freleased
+      (MAP: opt_view_map released freleased)
+    :
+      msg_map (Message.full val released) (Message.full val freleased)
+  .
+
+  Inductive tevent_map: ThreadEvent.t -> ThreadEvent.t -> Prop :=
+  | tevent_map_promise
+      loc from ffrom to fto msg fmsg kind
+      (FROM: f loc from ffrom)
+      (TO: f loc to fto)
+      (MSG: msg_map msg fmsg)
+    :
+      tevent_map
+        (ThreadEvent.promise loc from to msg kind)
+        (ThreadEvent.promise loc ffrom fto fmsg kind)
+  | tevent_map_read
+      loc to fto val released freleased ordr
+      (TO: f loc to fto)
+      (RELEASED: opt_view_map released freleased)
+    :
+      tevent_map
+        (ThreadEvent.read loc to val released ordr)
+        (ThreadEvent.read loc fto val freleased ordr)
+  | tevent_map_write
+      loc from ffrom to fto val released freleased ordw
+      (FROM: f loc from ffrom)
+      (TO: f loc to fto)
+      (RELEASED: opt_view_map released freleased)
+    :
+      tevent_map
+        (ThreadEvent.write loc from to val released ordw)
+        (ThreadEvent.write loc ffrom fto val freleased ordw)
+  | tevent_map_update
+      loc from ffrom to fto valr valw releasedr freleasedr releasedw freleasedw ordr ordw
+      (FROM: f loc from ffrom)
+      (TO: f loc to fto)
+      (RELEASEDR: opt_view_map releasedr freleasedr)
+      (RELEASEDW: opt_view_map releasedw freleasedw)
+    :
+      tevent_map
+        (ThreadEvent.update loc from to valr valw releasedr releasedr ordr ordw)
+        (ThreadEvent.update loc ffrom fto valr valw freleasedr freleasedw ordr ordw)
+  | tevent_map_fence
+      or ow
+    :
+      tevent_map
+        (ThreadEvent.fence or ow)
+        (ThreadEvent.fence or ow)
+  | tevent_map_syscall
+      e
+    :
+      tevent_map
+        (ThreadEvent.syscall e)
+        (ThreadEvent.syscall e)
+  | tevent_map_silent
+    :
+      tevent_map
+        (ThreadEvent.silent)
+        (ThreadEvent.silent)
+  .
+
+  Definition non_collapsable (loc: Loc.t) (to: Time.t): Prop :=
+    forall to' (TLE: Time.lt to' to),
+      ~ collapsed loc to' to.
+
+  Lemma map_lt_non_collapsable
+        loc t0 t1 ft0 ft1
+        (MAP0: f loc t0 ft0)
+        (MAP1: f loc t1 ft1)
+        (NCLPS: non_collapsable loc t1)
+    :
+      Time.lt t0 t1 <-> Time.lt ft0 ft1.
+  Proof.
+    split; i.
+    - erewrite <- map_lt_iff; eauto.
+    - eapply map_lt_only_if; eauto.
+  Qed.
+
+  Inductive memory_map m fm: Prop :=
+  | memory_map_intro
+      (MAPPED: forall loc to from msg (GET: Memory.get loc to m = Some (from, msg)),
+          exists fto ffrom fmsg' fmsg,
+            (<<TO: f loc to fto>>) /\
+            (<<MSG: msg_map msg fmsg'>>) /\
+            (<<MSGLE: Message.le fmsg fmsg'>>) /\
+            (<<GET: Memory.get loc fto fm = Some (ffrom, fmsg)>>))
+      (ONLY: forall loc fto ffrom fmsg
+                    (GET: Memory.get loc fto fm = Some (ffrom, fmsg)),
+          exists to from msg,
+            (<<TO: f loc to fto>>) /\
+            (<<GET: Memory.get loc to m = Some (from, msg)>>) /\
+            (<<FROM: f loc from ffrom>>))
+  .
+
+  Inductive promises_map m fm: Prop :=
+  | promises_map_intro
+      (MAPPED: forall loc to from msg (GET: Memory.get loc to m = Some (from, msg)),
+          exists fto ffrom fmsg,
+            (<<NCLPS: non_collapsable loc to>>) /\
+            (<<TO: f loc to fto>>) /\
+            (<<MSG: msg_map msg fmsg>>) /\
+            (<<GET: Memory.get loc fto fm = Some (ffrom, fmsg)>>))
+      (ONLY: forall loc fto ffrom fmsg
+                    (GET: Memory.get loc fto fm = Some (ffrom, fmsg)),
+          exists to from msg,
+            (<<TO: f loc to fto>>) /\
+            (<<GET: Memory.get loc to m = Some (from, msg)>>) /\
+            (<<FROM: f loc from ffrom>>))
+  .
+
+  Lemma promises_map_memory_map m fm
+        (PROMISES: promises_map m fm)
+    :
+      memory_map m fm.
+  Proof.
+    inv PROMISES. econs; eauto.
+    i. exploit MAPPED; eauto. i. des.
+    esplits; eauto. refl.
+  Qed.
+  Hint Resolve promises_map_memory_map.
+
+  (* Inductive memory_map m fm: Prop := *)
+  (* | memory_map_intro *)
+  (*     (MAPPED: forall loc to from msg (GET: Memory.get loc to m = Some (from, msg)), *)
+  (*         exists fto ffrom fmsg, *)
+  (*           (<<TO: f loc to fto>>) /\ *)
+  (*           (<<MSG: msg_map msg fmsg>>) /\ *)
+  (*           (<<GET: Memory.get loc fto fm = Some (ffrom, fmsg)>>)) *)
+  (*     (ONLY: forall loc fto ffrom fmsg *)
+  (*                   (GET: Memory.get loc fto fm = Some (ffrom, fmsg)), *)
+  (*         exists to from msg, *)
+  (*           (<<TO: f loc to fto>>) /\ *)
+  (*           (<<GET: Memory.get loc to m = Some (from, msg)>>)) *)
+  (* . *)
+
+  (* Record promises_map (prom fprom: Memory.t): Prop := *)
+  (*   promises_map_intro *)
+  (*     { promises_memory_map: memory_map prom fprom; *)
+  (*       promises_non_collapsable: *)
+  (*         forall loc to from msg *)
+  (*                (GET: Memory.get loc to prom = Some (from, msg)), *)
+  (*           non_collapsable loc to; } *)
+  (* . *)
+
+  Lemma time_join_map loc t0 t1 ft0 ft1
+        (MAP0: f loc t0 ft0)
+        (MAP1: f loc t1 ft1)
+    :
+      f loc (Time.join t0 t1) (Time.join ft0 ft1).
   Proof.
     unfold Time.join. des_ifs.
-    - eapply map_preserving_le_if in l; eauto. timetac.
+    - eapply map_le in l; eauto. timetac.
     - destruct l0; auto.
-      eapply map_preserving_lt_only_if in H; eauto.
-      exfalso. eapply Time.lt_strorder. etrans; eauto.
+      + eapply map_lt_only_if in H; eauto.
+        exfalso. eapply Time.lt_strorder. etrans; eauto.
+      + destruct H. auto.
   Qed.
 
-  Lemma map_timemap_bot P f
-        (PRSV: map_preserving P f)
+  Lemma timemap_bot_map
     :
-      timemap_map f TimeMap.bot = TimeMap.bot.
+      timemap_map TimeMap.bot TimeMap.bot.
   Proof.
-    extensionality loc. unfold timemap_map.
-    erewrite map_preserving_bot; eauto.
+    ii. eapply map_bot.
   Qed.
 
-  Lemma map_view_bot P f
-        (PRSV: map_preserving P f)
+  Lemma view_bot_map
     :
-      view_map f View.bot = View.bot.
+      view_map View.bot View.bot.
   Proof.
-    unfold view_map, View.bot. ss. f_equal.
-    - eapply map_timemap_bot; eauto.
-    - eapply map_timemap_bot; eauto.
+    econs.
+    - eapply timemap_bot_map; eauto.
+    - eapply timemap_bot_map; eauto.
   Qed.
 
-  Lemma map_timemap_singleton f P loc to
-        (INMEMORY: map_preserving P f)
-        (CLOSED2: P loc to)
+  Lemma timemap_singleton_map loc to fto
+        (MAP: f loc to fto)
     :
-      timemap_map f (TimeMap.singleton loc to) =
-      TimeMap.singleton loc (f loc to).
+      timemap_map (TimeMap.singleton loc to) (TimeMap.singleton loc fto).
   Proof.
-    extensionality l.
-    unfold timemap_map, TimeMap.singleton.
+    ii. unfold TimeMap.singleton.
     setoid_rewrite LocFun.add_spec. des_ifs.
-    rewrite LocFun.init_spec. erewrite map_preserving_bot; eauto.
   Qed.
 
-  Lemma map_singleton_ur f P loc to
-        (INMEMORY: map_preserving P f)
-        (CLOSED2: P loc to)
+  Lemma singleton_ur_map loc to fto
+        (MAP: f loc to fto)
     :
-      view_map f (View.singleton_ur loc to) =
-      View.singleton_ur loc (f loc to).
+      view_map (View.singleton_ur loc to) (View.singleton_ur loc fto).
   Proof.
-    unfold view_map, View.singleton_ur. ss.
-    erewrite map_timemap_singleton; eauto.
+    unfold View.singleton_ur. econs; ss.
+    - eapply timemap_singleton_map; eauto.
+    - eapply timemap_singleton_map; eauto.
   Qed.
 
-  Lemma map_singleton_rw f P loc to
-        (INMEMORY: map_preserving P f)
-        (CLOSED2: P loc to)
+  Lemma singleton_rw_map loc to fto
+        (MAP: f loc to fto)
     :
-      view_map f (View.singleton_rw loc to) =
-      View.singleton_rw loc (f loc to).
+      view_map (View.singleton_rw loc to) (View.singleton_rw loc fto).
   Proof.
-    unfold view_map, View.singleton_rw. ss.
-    erewrite map_timemap_singleton; eauto. f_equal.
-    eapply map_timemap_bot; eauto.
+    unfold View.singleton_ur. econs; ss.
+    eapply timemap_singleton_map; eauto.
   Qed.
 
-  Lemma map_singleton_ur_if f P loc to cond
-        (INMEMORY: map_preserving P f)
-        (CLOSED2: P loc to)
+  Lemma singleton_ur_if_map loc to fto cond
+        (MAP: f loc to fto)
     :
-      view_map f (View.singleton_ur_if cond loc to) =
-      View.singleton_ur_if cond loc (f loc to).
+      view_map (View.singleton_ur_if cond loc to) (View.singleton_ur_if cond loc fto).
   Proof.
-    unfold view_map, View.singleton_ur_if. des_ifs.
-    - erewrite <- map_singleton_ur; eauto.
-    - erewrite <- map_singleton_rw; eauto.
+    unfold View.singleton_ur_if. des_ifs.
+    - eapply singleton_ur_map; eauto.
+    - eapply singleton_rw_map; eauto.
   Qed.
+
+  Lemma timemap_join_map tm0 tm1 ftm0 ftm1
+        (TM0: timemap_map tm0 ftm0)
+        (TM1: timemap_map tm1 ftm1)
+    :
+      timemap_map (TimeMap.join tm0 tm1) (TimeMap.join ftm0 ftm1).
+  Proof.
+    ii. unfold TimeMap.join.
+    eapply time_join_map; eauto.
+  Qed.
+
+  Lemma timemap_le_map tm0 tm1 ftm0 ftm1
+        (TM0: timemap_map tm0 ftm0)
+        (TM1: timemap_map tm1 ftm1)
+        (TMLE: TimeMap.le tm0 tm1)
+    :
+      TimeMap.le ftm0 ftm1.
+  Proof.
+    ii. eapply map_le; eauto.
+  Qed.
+
+  Lemma closed_timemap_map m fm tm ftm
+        (MEM: memory_map m fm)
+        (TM: timemap_map tm ftm)
+        (CLOSED: Memory.closed_timemap tm m)
+    :
+      Memory.closed_timemap ftm fm.
+  Proof.
+    inv MEM. ii. specialize (CLOSED loc). des.
+    eapply MAPPED in CLOSED. des. inv MSG.
+    specialize (TM loc).
+    hexploit (map_eq TM TO). i. subst.
+    inv MSGLE. esplits; eauto.
+  Qed.
+
+  Lemma closed_view_map m fm vw fvw
+        (MEM: memory_map m fm)
+        (VIEW: view_map vw fvw)
+        (CLOSED: Memory.closed_view vw m)
+    :
+      Memory.closed_view fvw fm.
+  Proof.
+    inv CLOSED. inv VIEW. econs.
+    - eapply closed_timemap_map; eauto.
+    - eapply closed_timemap_map; eauto.
+  Qed.
+
+  Lemma closed_opt_view_map m fm vw fvw
+        (MEM: memory_map m fm)
+        (VIEW: opt_view_map vw fvw)
+        (CLOSED: Memory.closed_opt_view vw m)
+    :
+      Memory.closed_opt_view fvw fm.
+  Proof.
+    inv CLOSED.
+    - inv VIEW. econs. eapply closed_view_map; eauto.
+    - inv VIEW. econs.
+  Qed.
+
+  Lemma view_join_map v0 v1 fv0 fv1
+        (VIEW0: view_map v0 fv0)
+        (VIEW1: view_map v1 fv1)
+    :
+      view_map (View.join v0 v1) (View.join fv0 fv1).
+  Proof.
+    inv VIEW0. inv VIEW1.
+    unfold View.join. econs; ss.
+    - eapply timemap_join_map; eauto.
+    - eapply timemap_join_map; eauto.
+  Qed.
+
+  Lemma tviewjoin_map tv0 tv1 ftv0 ftv1
+        (TVIEW0: tview_map tv0 ftv0)
+        (TVIEW1: tview_map tv1 ftv1)
+    :
+      tview_map (TView.join tv0 tv1) (TView.join ftv0 ftv1).
+  Proof.
+    inv TVIEW0. inv TVIEW1.
+    unfold TView.join. econs; ss.
+    - i. eapply view_join_map; eauto.
+    - eapply view_join_map; eauto.
+    - eapply view_join_map; eauto.
+  Qed.
+
+  Lemma unwrap_map released freleased
+        (VIEW: opt_view_map released freleased)
+    :
+      view_map (View.unwrap released) (View.unwrap freleased).
+  Proof.
+    inv VIEW; ss.
+  Qed.
+
+  Lemma readable_map vw fvw loc to fto released freleased ordr
+        (VIEW: view_map vw fvw)
+        (TO: f loc to fto)
+        (RELEASED: opt_view_map released freleased)
+        (READABLE: TView.readable vw loc to released ordr)
+    :
+      TView.readable fvw loc fto freleased ordr.
+  Proof.
+    inv READABLE. econs.
+    - eapply map_le; eauto.
+      inv VIEW. eauto.
+    - intros ORD. specialize (RLX ORD).
+      eapply map_le; eauto.
+      inv VIEW. eauto.
+  Qed.
+
+  Lemma read_tview_map tvw ftvw loc to fto released freleased ord
+        (TVIEW: tview_map tvw ftvw)
+        (TO: f loc to fto)
+        (RELEASED: opt_view_map released freleased)
+    :
+      tview_map
+        (TView.read_tview tvw loc to released ord)
+        (TView.read_tview ftvw loc fto freleased ord).
+  Proof.
+    unfold TView.read_tview. econs; ss.
+    - i. eapply map_rel; eauto.
+    - eapply view_join_map.
+      + eapply view_join_map.
+        * eapply map_cur; eauto.
+        * eapply singleton_ur_if_map; eauto.
+      + des_ifs. eapply unwrap_map; eauto.
+    - eapply view_join_map.
+      + eapply view_join_map.
+        * eapply map_acq; eauto.
+        * eapply singleton_ur_if_map; eauto.
+      + des_ifs. eapply unwrap_map; eauto.
+  Qed.
+
+  Lemma write_tview_map tvw ftvw sc fsc loc to fto ord
+        (TVIEW: tview_map tvw ftvw)
+        (TO: f loc to fto)
+    :
+      tview_map
+        (TView.write_tview tvw sc loc to ord)
+        (TView.write_tview ftvw fsc loc fto ord).
+  Proof.
+    unfold TView.write_tview. econs; ss.
+    - i. setoid_rewrite LocFun.add_spec. des_ifs.
+      + eapply view_join_map.
+        * eapply map_cur; eauto.
+        * eapply singleton_ur_map; eauto.
+      + eapply view_join_map.
+        * eapply map_rel; eauto.
+        * eapply singleton_ur_map; eauto.
+      + eapply map_rel in TVIEW. eauto.
+    - eapply view_join_map.
+      + eapply map_cur; eauto.
+      + eapply singleton_ur_map; eauto.
+    - eapply view_join_map.
+      + eapply map_acq; eauto.
+      + eapply singleton_ur_map; eauto.
+  Qed.
+
+  Lemma read_fence_tview_map tvw ftvw ord
+        (TVIEW: tview_map tvw ftvw)
+    :
+      tview_map
+        (TView.read_fence_tview tvw ord)
+        (TView.read_fence_tview ftvw ord).
+  Proof.
+    unfold TView.read_fence_tview. econs; ss.
+    - i. eapply map_rel; eauto.
+    - des_ifs.
+      + eapply map_acq; eauto.
+      + eapply map_cur; eauto.
+    - eapply map_acq; eauto.
+  Qed.
+
+  Lemma write_fence_sc_map tvw ftvw sc fsc ord
+        (TVIEW: tview_map tvw ftvw)
+        (SC: timemap_map sc fsc)
+    :
+      timemap_map
+        (TView.write_fence_sc tvw sc ord)
+        (TView.write_fence_sc ftvw fsc ord).
+  Proof.
+    unfold TView.write_fence_sc. des_ifs.
+    eapply timemap_join_map; eauto.
+    eapply map_rlx; eauto. eapply map_cur; eauto.
+  Qed.
+
+  Lemma write_fence_tview_map tvw ftvw sc fsc ord
+        (TVIEW: tview_map tvw ftvw)
+        (SC: timemap_map sc fsc)
+    :
+      tview_map
+        (TView.write_fence_tview tvw sc ord)
+        (TView.write_fence_tview ftvw fsc ord).
+  Proof.
+    unfold TView.write_fence_tview. econs; ss.
+    - i. des_ifs.
+      + econs; ss.
+        * eapply write_fence_sc_map; eauto.
+        * eapply write_fence_sc_map; eauto.
+      + eapply map_cur; eauto.
+      + eapply map_rel; eauto.
+    - des_ifs.
+      + econs; ss.
+        * eapply write_fence_sc_map; eauto.
+        * eapply write_fence_sc_map; eauto.
+      + eapply map_cur; eauto.
+    - eapply view_join_map.
+      + eapply map_acq; eauto.
+      + des_ifs. econs; ss.
+        * eapply write_fence_sc_map; eauto.
+        * eapply write_fence_sc_map; eauto.
+  Qed.
+
+  Lemma write_released_map tvw ftvw sc fsc loc to fto released freleased ord
+        (TVIEW: tview_map tvw ftvw)
+        (SC: timemap_map sc fsc)
+        (TO: f loc to fto)
+        (VIEW: opt_view_map released freleased)
+    :
+      opt_view_map
+        (TView.write_released tvw sc loc to released ord)
+        (TView.write_released ftvw fsc loc fto freleased ord).
+  Proof.
+    unfold TView.write_released. des_ifs; econs.
+    eapply view_join_map; eauto.
+    - eapply unwrap_map; eauto.
+    - eapply map_rel; eauto. eapply write_tview_map; eauto.
+  Qed.
+
+  Lemma bot_promises_map fprom
+        (MEM: promises_map Memory.bot fprom)
+    :
+      fprom = Memory.bot.
+  Proof.
+    inv MEM. eapply Memory.ext. i.
+    rewrite Memory.bot_get.
+    destruct (Memory.get loc ts fprom) eqn:GET; auto.
+    destruct p. eapply ONLY in GET. des.
+    rewrite Memory.bot_get in GET; eauto. clarify.
+  Qed.
+
+  Lemma msg_get_map m fm loc to from msg
+        (MEM: memory_map m fm)
+        (GET: Memory.get loc to m = Some (from, msg))
+    :
+      exists ffrom fto fmsg fmsg',
+        (<<GET: Memory.get loc fto fm = Some (ffrom, fmsg)>>) /\
+        (<<TO: f loc to fto>>) /\
+        (<<MSG: msg_map msg fmsg'>>) /\
+        (<<MSGLE: Message.le fmsg fmsg'>>).
+  Proof.
+    inv MEM. eapply MAPPED in GET. des. esplits; eauto.
+  Qed.
+
+  Lemma msg_get_map_if m fm loc to fto from msg
+        (MEM: memory_map m fm)
+        (TO: f loc to fto)
+        (GET: Memory.get loc to m = Some (from, msg))
+    :
+      exists ffrom fmsg fmsg',
+        (<<GET: Memory.get loc fto fm = Some (ffrom, fmsg)>>) /\
+        (<<MSG: msg_map msg fmsg'>>) /\
+        (<<MSGLE: Message.le fmsg fmsg'>>).
+  Proof.
+    inv MEM. eapply MAPPED in GET. des.
+    hexploit (map_eq TO TO0). i. subst.
+    esplits; eauto.
+  Qed.
+
+  Lemma msg_get_map_only_if m fm
+        (MEM: memory_map m fm)
+        loc fto ffrom fmsg
+        (GET: Memory.get loc fto fm = Some (ffrom, fmsg))
+    :
+      exists to from msg fmsg',
+        (<<TO: f loc to fto>>) /\
+        (<<GET: Memory.get loc to m = Some (from, msg)>>) /\
+        (<<FROM: f loc from ffrom>>) /\
+        (<<MSG: msg_map msg fmsg'>>) /\
+        (<<MSGLE: Message.le fmsg fmsg' >>)
+  .
+  Proof.
+    inv MEM.
+    dup GET. eapply ONLY in GET. des.
+    dup GET. eapply MAPPED in GET1. des.
+    hexploit (map_eq TO TO0). i. clarify.
+    esplits; eauto.
+  Qed.
+
+  Lemma promise_consistent_map tvw ftvw prom fprom
+        (TVIEW: tview_map tvw ftvw)
+        (PROMS: promises_map prom fprom)
+        (CONSISTENT: Local.promise_consistent (Local.mk tvw prom))
+    :
+      Local.promise_consistent (Local.mk ftvw fprom).
+  Proof.
+    ii. ss.
+    inv PROMS. exploit ONLY; eauto. i. des.
+    exploit MAPPED; eauto. i. des.
+    hexploit (map_eq TO TO0). i. clarify.
+    inv MSG. exploit CONSISTENT; ss; eauto.
+    i. erewrite <- map_lt_iff; eauto.
+    eapply map_rlx. eapply map_cur. auto.
+  Qed.
+
+  Lemma nonsynch_loc_map loc prom fprom
+        (PROMS: promises_map prom fprom)
+        (NONSYNCH: Memory.nonsynch_loc loc prom)
+    :
+      Memory.nonsynch_loc loc fprom.
+  Proof.
+    ii. dup GET.
+    inv PROMS. exploit ONLY; eauto. i. des.
+    exploit MAPPED; eauto. i. des.
+    hexploit (map_eq TO TO0). i. clarify.
+    eapply NONSYNCH in GET1. des_ifs.
+    - inv MSG. inv MAP. ss.
+    - inv MSG.
+  Qed.
+
+  Lemma writable_map vw fvw sc fsc loc to fto released freleased ordw
+        (VIEW: view_map vw fvw)
+        (TO: f loc to fto)
+        (RELEASED: opt_view_map released freleased)
+        (NCLPS: non_collapsable loc to)
+        (WRITABLE: TView.writable vw sc loc to ordw)
+    :
+      TView.writable fvw fsc loc fto ordw.
+  Proof.
+    inv WRITABLE. econs.
+    erewrite <- map_lt_non_collapsable; eauto.
+    eapply map_rlx. eauto.
+  Qed.
+
+  Lemma timemap_map_exists mem fmem tm
+        (MEM: memory_map mem fmem)
+        (CLOSED: Memory.closed_timemap tm mem)
+    :
+      exists ftm,
+        (<<TM: timemap_map tm ftm>>) /\
+        (<<CLOSED: Memory.closed_timemap ftm fmem>>).
+  Proof.
+    hexploit (choice (fun loc to =>
+                        (<<MAP: f loc (tm loc) to>>) /\
+                        exists from val released,
+                          Memory.get loc to fmem = Some (from, Message.full val released))).
+    { intros loc. specialize (CLOSED loc). des.
+      inv MEM. eapply MAPPED in CLOSED. des. inv MSG. inv MSGLE.
+      esplits; eauto. }
+    i. des. esplits; eauto.
+    - ii. specialize (H loc). des. eauto.
+    - ii. specialize (H loc). des. eauto.
+  Qed.
+
+  Lemma opt_view_map_exists mem fmem vw
+        (MEM: memory_map mem fmem)
+        (CLOSED: Memory.closed_opt_view vw mem)
+    :
+      exists fvw,
+        (<<VIEW: opt_view_map vw fvw>>) /\
+        (<<CLOSED: Memory.closed_opt_view fvw fmem>>).
+  Proof.
+    inv CLOSED.
+    - inv CLOSED0.
+      hexploit (timemap_map_exists MEM PLN). i. des.
+      hexploit (timemap_map_exists MEM RLX). i. des.
+      exists (Some (View.mk ftm ftm0)). esplits; eauto.
+      econs. econs; eauto.
+    - exists None. esplits; eauto. econs.
+  Qed.
+
+  Lemma msg_map_exists mem fmem msg
+        (MEM: memory_map mem fmem)
+        (CLOSED: Memory.closed_message msg mem)
+    :
+      exists fmsg,
+        (<<MSG: msg_map msg fmsg>>) /\
+        (<<CLOSED: Memory.closed_message fmsg fmem>>).
+  Proof.
+    inv CLOSED.
+    - exploit opt_view_map_exists; eauto. i. des.
+      exists (Message.full val fvw).
+      esplits; eauto. econs; eauto.
+    - exists Message.reserve.
+      esplits; eauto. econs; eauto.
+  Qed.
+
+  Lemma add_succeed_wf mem1 loc from to msg mem2
+        (ADD: Memory.add mem1 loc from to msg mem2)
+    :
+      (<<DISJOINT: forall to2 from2 msg2
+                          (GET2: Memory.get loc to2 mem1 = Some (from2, msg2)),
+          Interval.disjoint (from, to) (from2, to2)>>) /\
+      (<<TO1: Time.lt from to>>) /\
+      (<<MSG_WF: Message.wf msg>>).
+  Proof.
+    inv ADD. inv ADD0. esplits; eauto.
+  Qed.
+
+  Lemma lower_succeed_wf mem1 loc from to msg1 msg2 mem2
+        (LOWER: Memory.lower mem1 loc from to msg1 msg2 mem2)
+    :
+      (<<GET: Memory.get loc to mem1 = Some (from, msg1)>>) /\
+      (<<TS: Time.lt from to>>) /\
+      (<<MSG_WF: Message.wf msg2>>) /\
+      (<<MSG_LE: Message.le msg2 msg1>>).
+  Proof.
+    inv LOWER. inv LOWER0. esplits; eauto.
+  Qed.
+
+  Lemma split_succeed_wf mem1 loc ts1 ts2 ts3 msg2 msg3 mem2
+        (SPLIT: Memory.split mem1 loc ts1 ts2 ts3 msg2 msg3 mem2)
+    :
+      (<<GET2: Memory.get loc ts3 mem1 = Some (ts1, msg3)>>) /\
+      (<<TS12: Time.lt ts1 ts2>>) /\
+      (<<TS23: Time.lt ts2 ts3>>) /\
+      (<<MSG_WF: Message.wf msg2>>).
+  Proof.
+    inv SPLIT. inv SPLIT0. esplits; eauto.
+  Qed.
+
+  Lemma view_wf_map vw fvw
+        (VIEW: view_map vw fvw)
+        (VIEWWF: View.wf vw)
+    :
+      View.wf fvw.
+  Proof.
+    inv VIEWWF. inv VIEW.
+    econs. eapply timemap_le_map; eauto.
+  Qed.
+
+  Lemma opt_view_wf_map vw fvw
+        (VIEW: opt_view_map vw fvw)
+        (VIEWWF: View.opt_wf vw)
+    :
+      View.opt_wf fvw.
+  Proof.
+    inv VIEWWF; inv VIEW; econs.
+    eapply view_wf_map; eauto.
+  Qed.
+
+  Lemma msg_wf_map msg fmsg
+        (MSG: msg_map msg fmsg)
+        (MSGWF: Message.wf msg)
+    :
+      Message.wf fmsg.
+  Proof.
+    inv MSGWF.
+    - inv MSG. econs; ss. eapply opt_view_wf_map; eauto.
+    - inv MSG. econs.
+  Qed.
+
+  Lemma disjoint_equivalent from0 to0 from1 to1
+    :
+      (<<INTERSECT: ~ Interval.disjoint (from0, to0) (from1, to1)>>) <->
+      ((<<TS0: Time.lt from0 to0>>) /\ (<<TS1: Time.lt from1 to1>>) /\
+       (<<TS0: Time.lt (Time.join from0 from1) (Time.meet to0 to1)>>)).
+  Proof.
+    split; i. des.
+    - unfold Interval.disjoint in H.
+      eapply not_all_ex_not in H. des.
+      dup H. eapply not_imply_elim in H. eapply not_imply_elim2 in H0.
+      apply NNPP in H0.
+      destruct H. destruct H0. ss. splits.
+      + eapply TimeFacts.lt_le_lt; eauto.
+      + eapply TimeFacts.lt_le_lt; eauto.
+      + unfold Time.join, Time.meet. des_ifs.
+        * eapply TimeFacts.lt_le_lt; eauto.
+        * eapply TimeFacts.lt_le_lt; eauto.
+        * eapply TimeFacts.lt_le_lt; eauto.
+        * eapply TimeFacts.lt_le_lt; eauto.
+    - des. ii. eapply H.
+      + instantiate (1:=Time.meet to0 to1). econs; ss.
+        * unfold Time.join, Time.meet in *. des_ifs.
+          eapply TimeFacts.le_lt_lt; eauto.
+        * eapply Time.meet_l.
+      + econs; ss.
+        * unfold Time.join, Time.meet in *. des_ifs.
+          etrans; eauto.
+        * eapply Time.meet_r.
+  Qed.
+
+  Lemma time_meet_map loc t0 t1 ft0 ft1
+        (MAP0: f loc t0 ft0)
+        (MAP1: f loc t1 ft1)
+    :
+      f loc (Time.meet t0 t1) (Time.meet ft0 ft1).
+  Proof.
+    unfold Time.meet. des_ifs.
+    - eapply map_le in l; eauto. timetac.
+    - destruct l0; auto.
+      + eapply map_lt_only_if in H; eauto.
+        exfalso. eapply Time.lt_strorder. etrans; eauto.
+      + destruct H. auto.
+  Qed.
+
+  Lemma disjoint_map loc from0 ffrom0 to0 fto0 from1 ffrom1 to1 fto1
+        (FROM0: f loc from0 ffrom0)
+        (TO0: f loc to0 fto0)
+        (FROM1: f loc from1 ffrom1)
+        (TO1: f loc to1 fto1)
+        (DISJOINT: Interval.disjoint (from0, to0) (from1, to1))
+    :
+      Interval.disjoint (ffrom0, fto0) (ffrom1, fto1).
+  Proof.
+    apply NNPP. ii. revert DISJOINT.
+    apply disjoint_equivalent. apply disjoint_equivalent in H. des.
+    splits.
+    - eapply map_lt_only_if; eauto.
+    - eapply map_lt_only_if; eauto.
+    - eapply map_lt_only_if; eauto.
+      + eapply time_join_map; eauto.
+      + eapply time_meet_map; eauto.
+  Qed.
+
+  Lemma msg_get_promises_map m fm loc to from msg
+        (MEM: promises_map m fm)
+        (GET: Memory.get loc to m = Some (from, msg))
+    :
+      exists ffrom fto fmsg,
+        (<<NCLPS: non_collapsable loc to>>) /\
+        (<<GET: Memory.get loc fto fm = Some (ffrom, fmsg)>>) /\
+        (<<FROM: f loc from ffrom>>) /\
+        (<<TO: f loc to fto>>) /\
+        (<<MSG: msg_map msg fmsg>>) /\
+        (<<UNIQUE:
+           forall to' (TO: f loc to' fto) frommsg
+                  (GET: Memory.get loc to' m = Some frommsg),
+             to = to'>>).
+  Proof.
+    inv MEM.
+    exploit MAPPED; eauto. i. des.
+    exploit ONLY; eauto. i. des.
+    exploit MAPPED; try apply GET1; eauto. i. des.
+    hexploit (map_eq TO0 TO1). i. subst.
+    destruct (Time.le_lt_dec to to0); [destruct l|].
+    - exfalso. exploit NCLPS0; eauto. econs; eauto.
+    - destruct H. clarify. esplits; eauto.
+      i. destruct frommsg. eapply MAPPED in GET. des.
+      destruct (Time.le_lt_dec to to'); [destruct l|]; auto.
+      + exfalso. exploit NCLPS1; eauto. econs; eauto.
+      + exfalso. exploit NCLPS; eauto. econs; eauto.
+    - exfalso. exploit NCLPS; eauto. econs; eauto.
+  Qed.
+
+  Lemma view_le_map vw0 vw1 fvw0 fvw1
+        (VIEW0: view_map vw0 fvw0)
+        (VIEW1: view_map vw1 fvw1)
+        (VIEWLE: View.le vw0 vw1)
+    :
+      View.le fvw0 fvw1.
+  Proof.
+    inv VIEWLE. econs; eauto.
+    - eapply timemap_le_map.
+      + eapply map_pln; eauto.
+      + eapply map_pln; eauto.
+      + eauto.
+    - eapply timemap_le_map.
+      + eapply map_rlx; eauto.
+      + eapply map_rlx; eauto.
+      + eauto.
+  Qed.
+
+  Lemma opt_view_le_map vw0 vw1 fvw0 fvw1
+        (VIEW0: opt_view_map vw0 fvw0)
+        (VIEW1: opt_view_map vw1 fvw1)
+        (VIEWLE: View.opt_le vw0 vw1)
+    :
+      View.opt_le fvw0 fvw1.
+  Proof.
+    inv VIEWLE.
+    - inv VIEW0. econs.
+    - inv VIEW0. inv VIEW1. econs.
+      eapply view_le_map; eauto.
+  Qed.
+
+  Lemma msg_le_map msg0 msg1 fmsg0 fmsg1
+        (MSG0: msg_map msg0 fmsg0)
+        (MSG1: msg_map msg1 fmsg1)
+        (MSGLE: Message.le msg1 msg0)
+    :
+      Message.le fmsg1 fmsg0.
+  Proof.
+    inv MSGLE.
+    - inv MSG0. inv MSG1. econs; eauto.
+      eapply opt_view_le_map; eauto.
+    - inv MSG0. econs; eauto.
+  Qed.
+
+  Lemma add_promises_map mem0 fmem0 loc from ffrom to fto msg fmsg mem1
+        (ADD: Memory.add mem0 loc from to msg mem1)
+        (PROMS: promises_map mem0 fmem0)
+        (FROM: f loc from ffrom)
+        (TO: f loc to fto)
+        (NCLPS: non_collapsable loc to)
+        (MSG: msg_map msg fmsg)
+    :
+      exists fmem1,
+        (<<PROMS: promises_map mem1 fmem1>>) /\
+        (<<ADD: Memory.add fmem0 loc ffrom fto fmsg fmem1>>).
+  Proof.
+    hexploit add_succeed_wf; eauto. i. des.
+    hexploit (@Memory.add_exists fmem0 loc ffrom fto fmsg).
+    { i. dup GET2. eapply msg_get_map_only_if in GET2; eauto. des.
+      eapply disjoint_map; eauto. }
+    { erewrite <- map_lt_non_collapsable; eauto. }
+    { eapply msg_wf_map; eauto. }
+    i. des. esplits; eauto.
+    econs.
+    - i. erewrite Memory.add_o in GET; eauto. des_ifs.
+      + ss. des; clarify.
+        esplits; eauto.
+        eapply Memory.add_get0; eauto.
+      + eapply msg_get_promises_map in GET; eauto.
+        guardH o. des. unguard.
+        esplits; eauto.
+        eapply Memory.add_get1; eauto.
+    - i. erewrite Memory.add_o in GET; eauto. des_ifs.
+      + ss. des; clarify. exists to. esplits; eauto.
+        eapply Memory.add_get0; eauto.
+      + eapply msg_get_map_only_if in GET; eauto.
+        guardH o. des. unguard.
+        exists to0. esplits; eauto.
+        eapply Memory.add_get1; eauto.
+  Qed.
+
+  Lemma lower_promises_map mem0 fmem0 loc from to msg0 msg1 fmsg1 mem1
+        (LOWER: Memory.lower mem0 loc from to msg0 msg1 mem1)
+        (MEM: promises_map mem0 fmem0)
+        (MSG: msg_map msg1 fmsg1)
+        (NCLPS: non_collapsable loc to)
+    :
+      exists ffrom fto fmsg0 fmem1,
+        (<<FROM: f loc from ffrom>>) /\
+        (<<TO: f loc to fto>>) /\
+        (<<MSG: msg_map msg0 fmsg0>>) /\
+        (<<MEM: promises_map mem1 fmem1>>) /\
+        (<<LOWER: Memory.lower fmem0 loc ffrom fto fmsg0 fmsg1 fmem1>>).
+  Proof.
+    exploit Memory.lower_get0; eauto. i. des.
+    hexploit lower_succeed_wf; eauto. i. des.
+    eapply msg_get_promises_map in GET; eauto. des.
+    hexploit (@Memory.lower_exists fmem0 loc ffrom fto fmsg fmsg1); eauto.
+    { erewrite <- map_lt_non_collapsable; eauto. }
+    { eapply msg_wf_map; eauto. }
+    { eapply msg_le_map; eauto. }
+    i. des. esplits; eauto.
+    econs.
+    - i. erewrite Memory.lower_o in GET2; eauto. des_ifs.
+      + ss. des; clarify.
+        esplits; eauto.
+        eapply Memory.lower_get0; eauto.
+      + eapply msg_get_promises_map in GET2; eauto.
+        guardH o. des. unguard.
+        exists fto0, ffrom0, fmsg0. esplits; eauto.
+        erewrite Memory.lower_o; eauto. des_ifs.
+        ss. des; clarify. exfalso. eauto.
+    - i. erewrite Memory.lower_o in GET2; eauto. des_ifs.
+      + ss. des; clarify.
+        esplits; eauto.
+      + dup MEM. inv MEM. eapply ONLY in GET2.
+        guardH o. des. unguard.
+        exists to0, from0, msg.
+        esplits; eauto. erewrite Memory.lower_o; eauto.
+        des_ifs. ss; des; clarify.
+        hexploit (map_eq TO0 TO). i. clarify.
+  Qed.
+
+  Lemma split_promises_map mem0 fmem0 loc ts1 ts2 ts3 msg0 msg1 fmsg0 mem1 fts2
+        (SPLIT: Memory.split mem0 loc ts1 ts2 ts3 msg0 msg1 mem1)
+        (MEM: promises_map mem0 fmem0)
+        (TS2: f loc ts2 fts2)
+        (MSG: msg_map msg0 fmsg0)
+        (NCLPS: non_collapsable loc ts2)
+    :
+      exists fts1 fts3 fmsg1 fmem1,
+        (<<TS1: f loc ts1 fts1>>) /\
+        (<<TS3: f loc ts3 fts3>>) /\
+        (<<MSG: msg_map msg1 fmsg1>>) /\
+        (<<MEM: promises_map mem1 fmem1>>) /\
+        (<<SPLIT: Memory.split fmem0 loc fts1 fts2 fts3 fmsg0 fmsg1 fmem1>>).
+  Proof.
+    exploit Memory.split_get0; eauto. i. des.
+    hexploit split_succeed_wf; eauto. i. des.
+    eapply msg_get_promises_map in GET3; eauto. des.
+    hexploit (@Memory.split_exists fmem0 loc ffrom fts2 fto fmsg0 fmsg); eauto.
+    { erewrite <- map_lt_non_collapsable; try apply TS12; eauto. }
+    { erewrite <- map_lt_non_collapsable; try apply TS23; eauto. }
+    { eapply msg_wf_map; eauto. }
+    i. des. esplits; eauto.
+    econs.
+    - i. erewrite Memory.split_o in GET4; eauto. des_ifs.
+      + ss. des; clarify.
+        exploit Memory.split_get0; eauto. i. des.
+        esplits; eauto.
+      + ss. des; clarify.
+        exploit Memory.split_get0; eauto. i. des.
+        esplits; eauto.
+      + eapply msg_get_promises_map in GET4; eauto.
+        guardH o. guardH o0. des. unguard.
+        exists fto0, ffrom0, fmsg1. esplits; eauto.
+        erewrite Memory.split_o; eauto.
+        des_ifs; ss; des; clarify.
+        * exploit Memory.split_get0; eauto. i. des. clarify.
+        * ss. des; clarify.
+          hexploit UNIQUE0; try apply TO; eauto.
+          i. clarify.
+    - i. erewrite Memory.split_o in GET4; eauto. des_ifs.
+      + ss. des; clarify.
+        esplits; eauto.
+      + ss. des; clarify.
+        esplits; eauto.
+      + dup MEM. inv MEM. eapply ONLY in GET4.
+        guardH o. guardH o0. des.
+        esplits; eauto.
+        erewrite Memory.split_o; eauto.
+        unguard. ss. des_ifs; ss; eauto.
+        * ss; des; clarify.
+        * ss; des; clarify. exfalso.
+          hexploit (map_eq TO0 TO). i. clarify.
+  Qed.
+
+  Lemma remove_promises_map mem0 fmem0 loc from to msg mem1
+        (REMOVE: Memory.remove mem0 loc from to msg mem1)
+        (MEM: promises_map mem0 fmem0)
+    :
+      exists ffrom fto fmsg fmem1,
+        (<<TO: f loc to fto>>) /\
+        (<<FROM: f loc from ffrom>>) /\
+        (<<MSG: msg_map msg fmsg>>) /\
+        (<<MEM: promises_map mem1 fmem1>>) /\
+        (<<REMOVE: Memory.remove fmem0 loc ffrom fto fmsg fmem1>>).
+  Proof.
+    exploit Memory.remove_get0; eauto. i. des.
+    eapply msg_get_promises_map in GET; eauto. des.
+    hexploit (@Memory.remove_exists fmem0 loc ffrom fto fmsg); eauto.
+    i. des. esplits; eauto.
+    econs.
+    - i. erewrite Memory.remove_o in GET1; eauto. des_ifs. ss.
+      dup GET1. eapply msg_get_promises_map in GET1; eauto.
+      guardH o. des. unguard.
+      exists fto0, ffrom0, fmsg0. esplits; eauto.
+      erewrite Memory.remove_o; eauto. des_ifs; ss. des; clarify.
+      exploit UNIQUE; eauto. i. clarify.
+    - i. erewrite Memory.remove_o in GET1; eauto. des_ifs.
+      dup MEM. inv MEM. eapply ONLY in GET1.
+      guardH o. des.
+      esplits; eauto.
+      erewrite Memory.remove_o; eauto.
+      unguard. ss. des_ifs; ss; eauto.
+      des; clarify. exfalso.
+      hexploit (map_eq TO0 TO). i. clarify.
+  Qed.
+
+  Lemma add_memory_map mem0 fmem0 loc from ffrom to fto msg fmsg' fmsg mem1
+        (ADD: Memory.add mem0 loc from to msg mem1)
+        (MEM: memory_map mem0 fmem0)
+        (FROM: f loc from ffrom)
+        (TO: f loc to fto)
+        (NCLPS: non_collapsable loc to)
+        (MSG: msg_map msg fmsg')
+        (MSGLE: Message.le fmsg fmsg')
+        (MSGWF: Message.wf fmsg)
+    :
+      exists fmem1,
+        (<<MEM: memory_map mem1 fmem1>>) /\
+        (<<ADD: Memory.add fmem0 loc ffrom fto fmsg fmem1>>).
+  Proof.
+    hexploit add_succeed_wf; eauto. i. des.
+    hexploit (@Memory.add_exists fmem0 loc ffrom fto fmsg).
+    { i. dup GET2. eapply msg_get_map_only_if in GET2; eauto. des.
+      eapply disjoint_map; eauto. }
+    { erewrite <- map_lt_non_collapsable; eauto. }
+    { auto. }
+    i. des. esplits; eauto.
+    econs.
+    - i. erewrite Memory.add_o in GET; eauto. des_ifs.
+      + ss. des; clarify.
+        esplits; eauto.
+        eapply Memory.add_get0; eauto.
+      + eapply msg_get_map in GET; eauto.
+        guardH o. des. unguard.
+        esplits; eauto.
+        eapply Memory.add_get1; eauto.
+    - i. erewrite Memory.add_o in GET; eauto. des_ifs.
+      + ss. des; clarify. exists to. esplits; eauto.
+        eapply Memory.add_get0; eauto.
+      + eapply msg_get_map_only_if in GET; eauto.
+        guardH o. des. unguard.
+        exists to0. esplits; eauto.
+        eapply Memory.add_get1; eauto.
+  Qed.
+
+
+  Lemma remove_memory_map mem0 fmem0 loc from to msg mem1
+        (REMOVE: Memory.remove mem0 loc from to msg mem1)
+        (MEM: memory_map mem0 fmem0)
+    :
+      exists ffrom fto fmsg fmem1,
+        (<<TO: f loc to fto>>) /\
+        (<<FROM: f loc from ffrom>>) /\
+        (<<MSG: msg_map msg fmsg>>) /\
+        (<<MEM: promises_map mem1 fmem1>>) /\
+        (<<REMOVE: Memory.remove fmem0 loc ffrom fto fmsg fmem1>>).
+  Proof.
+    exploit Memory.remove_get0; eauto. i. des.
+    eapply msg_get_promises_map in GET; eauto. des.
+    hexploit (@Memory.remove_exists fmem0 loc ffrom fto fmsg); eauto.
+    i. des. esplits; eauto.
+    econs.
+    - i. erewrite Memory.remove_o in GET1; eauto. des_ifs. ss.
+      dup GET1. eapply msg_get_promises_map in GET1; eauto.
+      guardH o. des. unguard.
+      exists fto0, ffrom0, fmsg0. esplits; eauto.
+      erewrite Memory.remove_o; eauto. des_ifs; ss. des; clarify.
+      exploit UNIQUE; eauto. i. clarify.
+    - i. erewrite Memory.remove_o in GET1; eauto. des_ifs.
+      dup MEM. inv MEM. eapply ONLY in GET1.
+      guardH o. des.
+      esplits; eauto.
+      erewrite Memory.remove_o; eauto.
+      unguard. ss. des_ifs; ss; eauto.
+      des; clarify. exfalso.
+      hexploit (map_eq TO0 TO). i. clarify.
+  Qed.
+
+
+
+    - i. esplits; eauto.
+
+      eapply
+
+      hexploit (map_eq TO TO0).
+
+      exfalso. eapply o. eapply UNIQUE0; eauto.
+      exploit (MAP
+
+      des_ifs; ss; des; clarify.
+      * exploit Memory.split_get0; eauto. i. des. clarify.
+      * ss. des; clarify.
+        hexploit UNIQUE0; try apply TO; eauto.
+        i. clarify.
+
+
+      exploit Memory.remove_get0; eauto. i. des.
+
+      ss. des; clarify.
+      * exploit Memory.remove_get0; eauto. i. des.
+        esplits; eauto.
+      + ss. des; clarify.
+        exploit Memory.remove_get0; eauto. i. des.
+        esplits; eauto.
+      + eapply msg_get_promises_map in GET4; eauto.
+        guardH o. guardH o0. des. unguard.
+        exists fto0, ffrom0, fmsg1. esplits; eauto.
+        erewrite Memory.split_o; eauto.
+        des_ifs; ss; des; clarify.
+        * exploit Memory.split_get0; eauto. i. des. clarify.
+        * ss. des; clarify.
+          hexploit UNIQUE0; try apply TO; eauto.
+          i. clarify.
+    - i. erewrite Memory.split_o in GET4; eauto. des_ifs.
+      + ss. des; clarify.
+        esplits; eauto.
+      + ss. des; clarify.
+        esplits; eauto.
+      + dup MEM. inv MEM. eapply ONLY in GET4.
+        guardH o. guardH o0. des.
+        esplits; eauto.
+        erewrite Memory.split_o; eauto.
+        unguard. ss. des_ifs; ss; eauto.
+        * ss; des; clarify.
+        * ss; des; clarify. exfalso.
+          hexploit (map_eq TO0 TO). i. clarify.
+  Qed.
+
+
+          ss; des; clarify. exfalso.
+          hexploit (map_eq TO0 TO). i. clarify.
+        *
+
+
+        * ss; des; clarify.
+
+                       des; clarify.
+
+
+        des_ifs; ss; des; clarify.
+
+
+        * unguard.
+
+          esplits; eauto.
+
+          erewrite Memory.split_o; eauto. des_ifs; ss; des; clarify.
+          admit.
+        *
+
+
+          admit.
+        * Memory.remove
+
+        exists to0, from0, msg.
+        esplits; eauto. erewrite Memory.lower_o; eauto.
+        des_ifs. ss; des; clarify.
+        hexploit (map_eq TO0 TO). i. clarify.
+  Qed.
+
+  Memory.promise
+
+    Memory.write
+
+        *
+
+
+        exists to0, from0, msg. esplits; eauto.
+
+        des.
+
+        eapply msg_get_promises_map in GET2; eauto.
+        guardH o. des. unguard.
+        exists fto0, ffrom0, fmsg0. esplits; eauto.
+        erewrite Memory.lower_o; eauto. des_ifs.
+        ss. des; clarify. exfalso. eauto.
+    - i.
+
+
+
+          ss. destruct a. clarify. hexploit UNIQUE; eauto.
+
+        des_ifs; des; ss; clarify.
+        * des; ss. clarify.
+
+
+          ss. des; clarify.
+
+        eapply Memory.lower_get1; eauto.
+    - i. erewrite Memory.add_o in GET; eauto. des_ifs.
+      + ss. des; clarify. exists to. esplits; eauto.
+        eapply Memory.add_get0; eauto.
+      + eapply msg_get_map_only_if in GET; eauto.
+        guardH o. des. unguard.
+        exists to0. esplits; eauto.
+        eapply Memory.add_get1; eauto.
+  Qed.
+
+
+
+  Lemma add_map mem0 fmem0 loc from ffrom to fto msg fmsg mem1
+        (ADD: Memory.add mem0 loc from to msg mem1)
+        (MEM: memory_map mem0 fmem0)
+        (FROM: f loc from ffrom)
+        (TO: f loc to fto)
+        (NCLPS: non_collapsable loc to)
+        (MSG: msg_map msg fmsg)
+    :
+      exists fmem1,
+        (<<MEM: memory_map mem1 fmem1>>) /\
+        (<<ADD: Memory.add fmem0 loc ffrom fto fmsg fmem1>>).
+  Proof.
+    hexploit add_succeed_wf; eauto. i. des.
+    hexploit (@Memory.add_exists fmem0 loc ffrom fto fmsg).
+    { i. dup GET2. eapply msg_get_map_only_if in GET2; eauto. des.
+      eapply disjoint_map; eauto. }
+    { erewrite <- map_lt_non_collapsable; eauto. }
+    { eapply msg_wf_map; eauto. }
+    i. des. esplits; eauto.
+    econs.
+    - i. erewrite Memory.add_o in GET; eauto. des_ifs.
+      + ss. des; clarify.
+        esplits; eauto.
+        eapply Memory.add_get0; eauto.
+      + eapply msg_get_map in GET; eauto.
+        guardH o. des. unguard.
+        esplits; eauto.
+        eapply Memory.add_get1; eauto.
+    - i. erewrite Memory.add_o in GET; eauto. des_ifs.
+      + ss. des; clarify. exists to. esplits; eauto.
+        eapply Memory.add_get0; eauto.
+      + eapply msg_get_map_only_if in GET; eauto.
+        guardH o. des. unguard.
+        exists to0. esplits; eauto.
+        eapply Memory.add_get1; eauto.
+  Qed.
+
+
+
+
+
+
+  Lemma lower_succeed_wf mem1 loc from to msg1 msg2 mem2
+        (LOWER: Memory.lower mem1 loc from to msg1 msg2 mem2)
+    :
+      (<<GET: Memory.get loc to mem1 = Some (from, msg1)>>) /\
+      (<<TS: Time.lt from to>>) /\
+      (<<MSG_WF: Message.wf msg2>>) /\
+      (<<MSG_LE: Message.le msg2 msg1>>).
+  Proof.
+    inv LOWER. inv LOWER0. esplits; eauto.
+  Qed.
+
+
+    hexploit add_succeed_wf; eauto. i. des.
+    hexploit (@Memory.add_exists fmem0 loc ffrom fto fmsg).
+    { i. dup GET2. eapply msg_get_map_only_if in GET2; eauto. des.
+      eapply disjoint_map; eauto. }
+    { erewrite <- map_lt_non_collapsable; eauto. }
+    { eapply msg_wf_map; eauto. }
+    i. des. esplits; eauto.
+    econs.
+    - i. erewrite Memory.add_o in GET; eauto. des_ifs.
+      + ss. des; clarify.
+        esplits; eauto.
+        eapply Memory.add_get0; eauto.
+      + eapply msg_get_map in GET; eauto.
+        guardH o. des. unguard.
+        esplits; eauto.
+        eapply Memory.add_get1; eauto.
+    - i. erewrite Memory.add_o in GET; eauto. des_ifs.
+      + ss. des; clarify. exists to. esplits; eauto.
+        eapply Memory.add_get0; eauto.
+      + eapply msg_get_map_only_if in GET; eauto.
+        guardH o. des. unguard.
+        exists to0. esplits; eauto.
+        eapply Memory.add_get1; eauto.
+  Qed.
+
+
+
+        (ADD
+        fmem0 ffrom fto
+
+  Memory.add
+
+  Lemma
+
+    des. destruct msg.
+    -
+
+
+Memory.promise
+Memory.closed_message
+
+Local.promise_step
+
+
 
   Definition respecting_memory (P: Loc.t -> Time.t -> Prop) (m: Memory.t) :=
     forall loc to from msg (GET: Memory.get loc to m = Some (from, msg)),
@@ -1748,7 +2936,7 @@ Section MAPPED.
 
   Lemma closed_timemap_respecting P m f tm
         (RESPECT: respecting_memory P m)
-        (PRSV: map_preserving P f)
+        (PRSV: prsv P f)
         (CLOSED: Memory.closed_timemap tm m)
     :
       respecting_map P tm.
@@ -1759,7 +2947,7 @@ Section MAPPED.
 
   Lemma closed_view_respecting P m f vw
         (RESPECT: respecting_memory P m)
-        (PRSV: map_preserving P f)
+        (PRSV: prsv P f)
         (CLOSED: Memory.closed_view vw m)
     :
       respecting_view P vw.
@@ -1771,7 +2959,7 @@ Section MAPPED.
 
   Lemma closed_opt_view_respecting P m f vw
         (RESPECT: respecting_memory P m)
-        (PRSV: map_preserving P f)
+        (PRSV: prsv P f)
         (CLOSED: Memory.closed_opt_view vw m)
     :
       respecting_opt_view P vw.
@@ -1783,7 +2971,7 @@ Section MAPPED.
 
   Lemma closed_tview_respecting P m f tvw
         (RESPECT: respecting_memory P m)
-        (PRSV: map_preserving P f)
+        (PRSV: prsv P f)
         (CLOSED: TView.closed tvw m)
     :
       respecting_tview P tvw.
@@ -1810,7 +2998,7 @@ Section MAPPED.
   Qed.
 
   Lemma map_timemap_join P f tm0 tm1
-        (PRSV: map_preserving P f)
+        (PRSV: prsv P f)
         (CLOSED0: respecting_map P tm0)
         (CLOSED1: respecting_map P tm1)
     :
@@ -1821,7 +3009,7 @@ Section MAPPED.
   Qed.
 
   Lemma map_viewjoin P f v0 v1
-        (PRSV: map_preserving P f)
+        (PRSV: prsv P f)
         (CLOSED0: respecting_view P v0)
         (CLOSED1: respecting_view P v1)
     :
@@ -1834,7 +3022,7 @@ Section MAPPED.
   Qed.
 
   Lemma map_tviewjoin P f tv0 tv1
-        (PRSV: map_preserving P f)
+        (PRSV: prsv P f)
         (CLOSED0: respecting_tview P tv0)
         (CLOSED1: respecting_tview P tv1)
     :
@@ -1848,7 +3036,7 @@ Section MAPPED.
   Qed.
 
   Lemma map_unwrap P f released
-        (PRSV: map_preserving P f)
+        (PRSV: prsv P f)
         (CLOSED0: respecting_opt_view P released)
     :
       view_map f (View.unwrap released) =
@@ -1896,7 +3084,7 @@ read_step (lc1 : Local.t) (mem1 : Memory.t) (loc : Loc.t) (to : Time.t)
   Local.write_step
 
   Lemma map_read_tview P f m v loc to released ord
-        (PRSV: map_preserving P f)
+        (PRSV: prsv P f)
         (INMEMORY: respecting_memory P m)
         (CLOSED0: TView.closed v m)
         (CLOSED1: Memory.closed_opt_view released m)
@@ -2628,7 +3816,6 @@ Section SHORTERMEMORY.
     exploit COMPLETE; eauto.
   Qed.
 
-  (* TODO: make threadevent le and force eventpredicate is closed under that? *)
   Lemma shorter_memory_write prom mem_src mem_tgt loc from1 to1 val released mem_tgt' from'
         (SHORTER: shorter_memory mem_src mem_tgt)
         (ADD: Memory.write Memory.bot mem_tgt loc from1 to1 val released prom mem_tgt' Memory.op_kind_add)
